src/program_logic/dist_weakestpre.v
@@ -31,8 +31,8 @@ Definition equal_global_inG ct : iProp Σ :=
   (∀ g ns κs, @global_state_interp _ _(perennial_irisG (fst ct) (snd ct)) g ns κs ∗-∗
                grove_global_state_interp g ns κs).
 
-Definition wpd (k : nat) (E: coPset) (cts: list (crashG Σ * pbundleG T Σ)) (es: list (expr Λ)) :=
+Definition wpd (k : nat) (E: coPset) (cts: list (crashG Σ * pbundleG T Σ)) (ers: list (expr Λ * expr Λ)) :=
  (□ (∀ ct, ⌜ ct ∈ cts ⌝ → equal_global_inG ct) ∧
- [∗ list] i↦ct;e ∈ cts;es, ∃ Φ Φrx Φinv, wpr NotStuck k (fst ct) (snd ct) E e e Φ Φinv Φrx)%I.
+ [∗ list] i↦ct;er ∈ cts;ers, ∃ Φ Φrx Φinv, wpr NotStuck k (fst ct) (snd ct) E (fst er) (snd er) Φ Φinv Φrx)%I.
 
 End wpd.
